theories/higher_order.v
@@ -86,11 +86,16 @@ else idtac) hltac1 ; aux xs
 end 
 in aux h0.
 
+
+Tactic Notation "prenex_higher_order_with_equations" :=
+ltac2:(Control.enter prenex_higher_order_with_equations).
+
+Section Tests.
+
 Lemma bar : forall (A B C : Type) (l : list A) (f : A -> B) (g : B -> C), 
 map g (map f l) = map (fun x => g (f x)) l.
 intros.
 induction l; Control.enter anonymous_funs_with_equations; Control.enter prenex_higher_order_with_equations.
 Abort.
 
-Tactic Notation "prenex_higher_order_with_equations" :=
-ltac2:(Control.enter prenex_higher_order_with_equations).
+End Tests.
